prover/theories/Named.v
@@ -522,6 +522,16 @@ Defined.
     | @nctx_app_r p' C' prf => npatt_app p' (named_subst_ctx C' p)
     end.
 
+    Inductive is_nsubpattern_of_ind : NamedPattern -> NamedPattern -> Prop :=
+    | nsub_eq ϕ₁ ϕ₂ : ϕ₁ = ϕ₂ -> is_nsubpattern_of_ind ϕ₁ ϕ₂
+    | nsub_app_l ϕ₁ ϕ₂ ϕ₃ : is_nsubpattern_of_ind ϕ₁ ϕ₂ -> is_nsubpattern_of_ind ϕ₁ (npatt_app ϕ₂ ϕ₃)
+    | nsub_app_r ϕ₁ ϕ₂ ϕ₃ : is_nsubpattern_of_ind ϕ₁ ϕ₃ -> is_nsubpattern_of_ind ϕ₁ (npatt_app ϕ₂ ϕ₃)
+    | nsub_imp_l ϕ₁ ϕ₂ ϕ₃ : is_nsubpattern_of_ind ϕ₁ ϕ₂ -> is_nsubpattern_of_ind ϕ₁ (npatt_imp ϕ₂ ϕ₃)
+    | nsub_imp_r ϕ₁ ϕ₂ ϕ₃ : is_nsubpattern_of_ind ϕ₁ ϕ₃ -> is_nsubpattern_of_ind ϕ₁ (npatt_imp ϕ₂ ϕ₃)
+    | nsub_exists x ϕ₁ ϕ₂ : is_nsubpattern_of_ind ϕ₁ ϕ₂ -> is_nsubpattern_of_ind ϕ₁ (npatt_exists x ϕ₂)
+    | nsub_mu X ϕ₁ ϕ₂ : is_nsubpattern_of_ind ϕ₁ ϕ₂ -> is_nsubpattern_of_ind ϕ₁ (npatt_mu X ϕ₂)
+    .
+
 (*
   Print well_formed_positive.
 
